Developing tactics. Minor fixes.

LambdaS5/coq/Interpreter.v
@@ -27,7 +27,6 @@ Open Scope string_scope.
 
 
 Implicit Type runs : runs_type.
-Implicit Type store : store. (* TODO search and destroy *)
 Implicit Type st : store.
 Implicit Type c : ctx.
 
@@ -60,11 +59,11 @@ Definition if_eval_return runs c st e (cont : store -> value -> result) : result
 (****** Closures handling ******)
 
 (* Evaluates all arguments, passing the store from one to the next. *)
-Definition eval_arg_list_aux runs c (arg_expr : expr) (cont : Store.store -> list value -> result) st (l : list value) : result :=
+Definition eval_arg_list_aux runs c (arg_expr : expr) (cont : store -> list value -> result) st (l : list value) : result :=
   if_eval_return runs c st arg_expr (fun st arg => cont st (arg::l)) 
 .
 
-Definition eval_arg_list runs c st (args_expr : list expr) (cont : Store.store -> list value -> result) : result :=
+Definition eval_arg_list runs c st (args_expr : list expr) (cont : store -> list value -> result) : result :=
   List.fold_right (eval_arg_list_aux runs c) (fun st args => cont st (rev args)) args_expr st nil
 .
 
@@ -73,7 +72,7 @@ Definition apply runs c st (f_loc : value) (args : list value) : result :=
   if_result_some res (fun f =>
       match f with
       | value_closure _id env args_names body =>
-        let (st, args_locs) := Store.add_values st args in
+        let (st, args_locs) := add_values st args in
         let res := add_parameters env args_names args_locs in
         if_result_some res (fun vh =>
           eval_cont_terminate runs vh st body)
@@ -96,12 +95,12 @@ Definition eval_id runs c st (name : string) : result :=
 (* if e_cond e_true else e_false.
 * Evaluate the condition and get the associated value, then evaluate
 * e_true or e_false depending on the value. *)
-Definition eval_if runs c store (e_cond e_true e_false : expr) : result :=
-  if_eval_return runs c store e_cond (fun store v =>
+Definition eval_if runs c st (e_cond e_true e_false : expr) : result :=
+  if_eval_return runs c st e_cond (fun st v =>
     assert_get_bool v (fun b =>
       if b
-      then eval_cont_terminate runs c store e_true
-      else eval_cont_terminate runs c store e_false
+      then eval_cont_terminate runs c st e_true
+      else eval_cont_terminate runs c st e_false
   ))
 .
 
@@ -114,18 +113,18 @@ Definition eval_seq runs c st (e1 e2 : expr) : result :=
 
 (* A tail-recursive helper for eval_object_properties, that constructs
 * the list of properties. *)
-Fixpoint eval_object_properties_aux runs c store (l : list (string * property)) (acc : object_properties) (cont : Store.store -> object_properties -> result) {struct l} : result :=
+Fixpoint eval_object_properties_aux runs c st (l : list (string * property)) (acc : object_properties) (cont : store -> object_properties -> result) {struct l} : result :=
   match l with
-  | nil => cont store acc
+  | nil => cont st acc
   | (name, property_data (data_intro value_expr writable_expr enumerable_expr configurable_expr)) :: tail =>
-    if_eval_return runs c store configurable_expr (fun store configurable_v =>
-      if_eval_return runs c store enumerable_expr (fun store enumerable_v =>
-        if_eval_return runs c store value_expr (fun store value_v =>
-          if_eval_return runs c store writable_expr (fun store writable_v =>
+    if_eval_return runs c st configurable_expr (fun st configurable_v =>
+      if_eval_return runs c st enumerable_expr (fun st enumerable_v =>
+        if_eval_return runs c st value_expr (fun st value_v =>
+          if_eval_return runs c st writable_expr (fun st writable_v =>
             assert_get_bool configurable_v (fun configurable =>
               assert_get_bool enumerable_v (fun enumerable => 
                 assert_get_bool writable_v (fun writable => 
-                  eval_object_properties_aux runs c store tail (Heap.write acc name (
+                  eval_object_properties_aux runs c st tail (Heap.write acc name (
                     attributes_data_of {|
                       attributes_data_value := value_v;
                       attributes_data_writable := writable;
@@ -133,13 +132,13 @@ Fixpoint eval_object_properties_aux runs c store (l : list (string * property)) 
                       attributes_data_configurable := configurable |}
                     )) cont))))))) 
   | (name, property_accessor (accessor_intro getter_expr setter_expr enumerable_expr configurable_expr)) :: tail =>
-    if_eval_return runs c store configurable_expr (fun store configurable_v =>
-      if_eval_return runs c store enumerable_expr (fun store enumerable_v =>
-        if_eval_return runs c store getter_expr (fun store getter_v =>
-          if_eval_return runs c store setter_expr (fun store setter_v =>
+    if_eval_return runs c st configurable_expr (fun st configurable_v =>
+      if_eval_return runs c st enumerable_expr (fun st enumerable_v =>
+        if_eval_return runs c st getter_expr (fun st getter_v =>
+          if_eval_return runs c st setter_expr (fun st setter_v =>
             assert_get_bool configurable_v (fun configurable =>
               assert_get_bool enumerable_v (fun enumerable => 
-                eval_object_properties_aux runs c store tail (Heap.write acc name (
+                eval_object_properties_aux runs c st tail (Heap.write acc name (
                   attributes_accessor_of {|
                     attributes_accessor_get := getter_v;
                     attributes_accessor_set := setter_v;
@@ -150,32 +149,32 @@ Fixpoint eval_object_properties_aux runs c store (l : list (string * property)) 
 .
 (* Reads a list of syntax trees of properties and converts it to a heap
 * bindable to an object. *)
-Definition eval_object_properties runs c store (l : list (string * property)) (cont : Store.store -> object_properties -> result) : result :=
-  eval_object_properties_aux runs c store l Heap.empty cont
+Definition eval_object_properties runs c st (l : list (string * property)) (cont : store -> object_properties -> result) : result :=
+  eval_object_properties_aux runs c st l Heap.empty cont
 .
 
 (* { [ attrs ] props }
 * Evaluate the primval attribute (if any), then the proto attribute (defaults
 * to Undefined), then properties. Finally, allocate a new object with the
 * computed values. *)
-Definition eval_object_decl runs c store (attrs : objattrs) (l : list (string * property)) : result :=
+Definition eval_object_decl runs c st (attrs : objattrs) (l : list (string * property)) : result :=
   let 'objattrs_intro class_expr extensible_expr prototype_expr code_expr primval_expr := attrs in
     (* Order of evaluation as in the paper: *)
-    if_eval_return runs c store class_expr (fun store class_v =>
-      if_eval_return runs c store extensible_expr (fun store extensible_v =>
-        if_eval_return runs c store prototype_expr (fun store prototype_v =>
-          if_eval_return runs c store code_expr (fun store code_v =>
-            if_eval_return runs c store primval_expr (fun store primval_v =>
+    if_eval_return runs c st class_expr (fun st class_v =>
+      if_eval_return runs c st extensible_expr (fun st extensible_v =>
+        if_eval_return runs c st prototype_expr (fun st prototype_v =>
+          if_eval_return runs c st code_expr (fun st code_v =>
+            if_eval_return runs c st primval_expr (fun st primval_v =>
               assert_get_string class_v (fun class => assert_get_bool extensible_v (fun extensible =>
-                eval_object_properties runs c store l (fun store props =>
-                  let (store, loc) := Store.add_object store {|
+                eval_object_properties runs c st l (fun st props =>
+                  let (st, loc) := add_object st {|
                     object_proto := prototype_v;
                     object_class := class;
                     object_extensible := extensible;
                     object_prim_value := primval_v;
                     object_properties_ := props;
                     object_code := code_v |}
-                  in result_value store loc
+                  in result_value st loc
           ))))))))
 .
 
@@ -187,20 +186,20 @@ Definition eval_object_decl runs c store (attrs : objattrs) (l : list (string * 
 * the getter with the arguments.
 * Note the arguments are evaluated even if they are not passed to any
 * function. *)
-Definition eval_get_field runs c store (left_expr right_expr arg_expr : expr) : result :=
-  if_eval_return runs c store left_expr (fun store left_loc =>
-    if_eval_return runs c store right_expr (fun store right_loc =>
-      if_eval_return runs c store arg_expr (fun store arg_loc =>
+Definition eval_get_field runs c st (left_expr right_expr arg_expr : expr) : result :=
+  if_eval_return runs c st left_expr (fun st left_loc =>
+    if_eval_return runs c st right_expr (fun st right_loc =>
+      if_eval_return runs c st arg_expr (fun st arg_loc =>
         assert_get_object_ptr left_loc (fun ptr =>
           assert_get_string right_loc (fun name =>
-            let res := get_property store ptr name in
+            let res := get_property st ptr name in
             if_result_some res (fun ret =>
               match ret with
-              | Some (attributes_data_of data) => result_value store (attributes_data_value data)
+              | Some (attributes_data_of data) => result_value st (attributes_data_value data)
               | Some (attributes_accessor_of (attributes_accessor_intro getter _ _ _)) =>
-                  apply runs c store getter (left_loc :: (arg_loc :: nil))
+                  apply runs c st getter (left_loc :: (arg_loc :: nil))
               | None =>
-                  result_value store value_undefined
+                  result_value st value_undefined
               end
   ))))))
 .
@@ -214,53 +213,53 @@ Definition eval_get_field runs c store (left_expr right_expr arg_expr : expr) : 
 * with the `new_val` prepended to the list.
 * Note the arguments are evaluated even if they are not passed to any
 * function. *)
-Definition eval_set_field runs c store (left_expr right_expr new_val_expr arg_expr : expr) : result :=
-  if_eval_return runs c store left_expr (fun store left_loc =>
-    if_eval_return runs c store right_expr (fun store right_loc =>
-      if_eval_return runs c store new_val_expr (fun store new_val =>
-        if_eval_return runs c store arg_expr (fun store arg_loc =>
+Definition eval_set_field runs c st (left_expr right_expr new_val_expr arg_expr : expr) : result :=
+  if_eval_return runs c st left_expr (fun st left_loc =>
+    if_eval_return runs c st right_expr (fun st right_loc =>
+      if_eval_return runs c st new_val_expr (fun st new_val =>
+        if_eval_return runs c st arg_expr (fun st arg_loc =>
           assert_get_object_ptr left_loc (fun left_ptr =>
             assert_get_string right_loc (fun name =>
-              if_result_some (get_property store left_ptr name) (fun ret =>
+              if_result_some (get_property st left_ptr name) (fun ret =>
                 match ret with
                 | Some (attributes_data_of data) =>
                   if attributes_data_writable data
-                  then change_object_property_cont store left_ptr name (fun prop cont =>
-                    assert_get_object_from_ptr store left_ptr (fun object =>
+                  then change_object_property_cont st left_ptr name (fun prop cont =>
+                    assert_get_object_from_ptr st left_ptr (fun object =>
                       match get_object_property object name with
                       | Some _ => 
                         let attrs := attributes_data_of (attributes_data_value_update data new_val) in
-                        cont store (Some attrs) new_val
+                        cont st (Some attrs) new_val
                       | None => 
                         let attrs := attributes_data_of (attributes_data_intro new_val true true true) in
-                        cont store (Some attrs) new_val
+                        cont st (Some attrs) new_val
                       end))
-                  else result_exception store (value_string "unwritable-field")
+                  else result_exception st (value_string "unwritable-field")
                 | Some (attributes_accessor_of (attributes_accessor_intro _ setter _ _)) =>
                     (* Note: pattr_setters don't get the new value. See https://github.com/brownplt/LambdaS5/issues/45 *)
-                    apply runs c store setter (left_loc :: arg_loc :: nil)
+                    apply runs c st setter (left_loc :: arg_loc :: nil)
                 | None => 
-                  assert_get_object_from_ptr store left_ptr (fun object =>
+                  assert_get_object_from_ptr st left_ptr (fun object =>
                     if object_extensible object 
-                    then change_object_property store left_ptr name (fun prop =>
+                    then change_object_property st left_ptr name (fun prop =>
                       let attrs := attributes_data_of (attributes_data_intro new_val true true true) in
-                      (store, Some attrs, new_val))
-                    else result_value store value_undefined)
+                      (st, Some attrs, new_val))
+                    else result_value st value_undefined)
                 end)))))))
 . (* get_object_property object name *)
 
-Definition eval_deletefield runs c store (left_expr right_expr : expr) : result :=
-  if_eval_return runs c store left_expr (fun store left_loc =>
-    if_eval_return runs c store right_expr (fun store right_loc =>
+Definition eval_deletefield runs c st (left_expr right_expr : expr) : result :=
+  if_eval_return runs c st left_expr (fun st left_loc =>
+    if_eval_return runs c st right_expr (fun st right_loc =>
       assert_get_object_ptr left_loc (fun left_ptr =>
         assert_get_string right_loc (fun name =>
-          change_object_cont store left_ptr (fun obj cont =>
+          change_object_cont st left_ptr (fun obj cont =>
             match get_object_property obj name with
             | Some attr => 
               if attributes_configurable attr 
-              then cont store (delete_object_property obj name) value_true
-              else result_exception store (value_string "unconfigurable-delete")
-            | None => cont store obj value_false
+              then cont st (delete_object_property obj name) value_true
+              else result_exception st (value_string "unconfigurable-delete")
+            | None => cont st obj value_false
             end
   )))))
 .
@@ -271,7 +270,7 @@ Definition eval_deletefield runs c store (left_expr right_expr : expr) : result 
 * Evaluate the body in the new store. *)
 Definition eval_let runs c st (id : string) (value_expr body_expr : expr) : result :=
   if_eval_return runs c st value_expr (fun st value =>
-      let (c, st) := Store.add_named_value c st id value in
+      let (c, st) := add_named_value c st id value in
         eval_cont_terminate runs c st body_expr
   )
 .
@@ -280,12 +279,12 @@ Definition eval_let runs c st (id : string) (value_expr body_expr : expr) : resu
 * Evaluate expr with a reference to itself, set it to a fresh location in the store,
 * and bind this location to the name `id` in the store.
 * Evaluate the body in the new store. *)
-Definition eval_rec runs c store (id : string) (value_expr body_expr : expr) : result :=
-  match Store.add_named_value_loc c store id value_undefined with
-  | (c, store, self_loc) =>
-    if_eval_return runs c store value_expr (fun store value =>
-      let store := Store.add_value_at_location store self_loc value in
-        eval_cont_terminate runs c store body_expr
+Definition eval_rec runs c st (id : string) (value_expr body_expr : expr) : result :=
+  match add_named_value_loc c st id value_undefined with
+  | (c, st, self_loc) =>
+    if_eval_return runs c st value_expr (fun st value =>
+      let st := add_value_at_location st self_loc value in
+        eval_cont_terminate runs c st body_expr
     )
   end
 .
@@ -293,18 +292,18 @@ Definition eval_rec runs c store (id : string) (value_expr body_expr : expr) : r
 (* name := expr
 * Evaluate expr, and set it at the location bound to `name`. Fail if `name`
 * is not associated with a location in the store. *)
-Definition eval_setbang runs c store (name : string) (expr : expr) : result :=
-  if_eval_return runs c store expr (fun store value =>
+Definition eval_setbang runs c st (name : string) (expr : expr) : result :=
+  if_eval_return runs c st expr (fun st value =>
     assert_get_loc c name (fun loc =>
-      result_value (Store.add_value_at_location store loc value) value
+      result_value (add_value_at_location st loc value) value
   ))
 .
 
 (* func (args) { body }
 * Capture the environment's name-to-location heap and return a closure. *)
 Definition eval_lambda runs c st (args : list id) (body : expr) : result :=
-  let (store, loc) := Store.add_closure c st args body in
-  result_value store loc
+  let (st, v) := add_closure c st args body in
+  result_value st v
 .
 
 (* f (args)
@@ -318,117 +317,117 @@ Definition eval_lambda runs c st (args : list id) (body : expr) : result :=
 * * else, `var` is left unchanged (ie. if it was mapped to a location,
 *   it still maps to this location; and if it did not map to anything,
 *   it still does not map to anything). *)
-Definition eval_app runs c store (f : expr) (args_expr : list expr) : result :=
-  if_eval_return runs c store f (fun store f_loc =>
-    eval_arg_list runs c store args_expr (fun store args =>
-      apply runs c store f_loc args
+Definition eval_app runs c st (f : expr) (args_expr : list expr) : result :=
+  if_eval_return runs c st f (fun st f_loc =>
+    eval_arg_list runs c st args_expr (fun st args =>
+      apply runs c st f_loc args
   ))
 .
 
 
 (* left[right<attr>] *)
-Definition eval_getattr runs c store left_expr right_expr attr :=
-  if_eval_return runs c store left_expr (fun store left_ =>
-    if_eval_return runs c store right_expr (fun store right_ =>
-      assert_get_object store left_ (fun obj =>
+Definition eval_getattr runs c st left_expr right_expr attr :=
+  if_eval_return runs c st left_expr (fun st left_ =>
+    if_eval_return runs c st right_expr (fun st right_ =>
+      assert_get_object st left_ (fun obj =>
         assert_get_string right_ (fun fieldname =>
           if_result_some (get_object_pattr obj fieldname attr) (fun v =>
-            result_value store v
+            result_value st v
   )))))
 .
 
 (* left[right<attr> = new_val] *)
-Definition eval_setattr runs c store left_expr right_expr attr new_val_expr :=
-  if_eval_return runs c store left_expr (fun store left_ =>
-    if_eval_return runs c store right_expr (fun store right_ =>
-      if_eval_return runs c store new_val_expr (fun store new_val =>
+Definition eval_setattr runs c st left_expr right_expr attr new_val_expr :=
+  if_eval_return runs c st left_expr (fun st left_ =>
+    if_eval_return runs c st right_expr (fun st right_ =>
+      if_eval_return runs c st new_val_expr (fun st new_val =>
         assert_get_object_ptr left_ (fun obj_ptr =>
           assert_get_string right_ (fun fieldname =>
-            change_object_cont store obj_ptr (fun obj cont =>
+            change_object_cont st obj_ptr (fun obj cont =>
               if_result_some (set_object_pattr obj fieldname attr new_val) (fun obj' =>
-                cont store obj' new_val
+                cont st obj' new_val
   )))))))
 .
 
-Definition eval_getobjattr runs c store obj_expr oattr :=
-  if_eval_return runs c store obj_expr (fun store obj_loc =>
-    assert_get_object store obj_loc (fun obj =>
-      result_value store (get_object_oattr obj oattr)))
+Definition eval_getobjattr runs c st obj_expr oattr :=
+  if_eval_return runs c st obj_expr (fun st obj_loc =>
+    assert_get_object st obj_loc (fun obj =>
+      result_value st (get_object_oattr obj oattr)))
 .
 
-Definition eval_setobjattr runs c store obj_expr oattr attr :=
-  if_eval_return runs c store obj_expr (fun store obj_loc =>
-    if_eval_return runs c store attr (fun store v =>
+Definition eval_setobjattr runs c st obj_expr oattr attr :=
+  if_eval_return runs c st obj_expr (fun st obj_loc =>
+    if_eval_return runs c st attr (fun st v =>
       assert_get_object_ptr obj_loc (fun obj_ptr =>
-        change_object_cont store obj_ptr (fun obj cont =>
+        change_object_cont st obj_ptr (fun obj cont =>
           if_result_some (set_object_oattr obj oattr v) (fun obj' =>
-            cont store obj' v)))))
+            cont st obj' v)))))
 .
 
-Definition eval_ownfieldnames runs c store obj_expr : result :=
-  if_eval_return runs c store obj_expr (fun store obj_loc =>
-    assert_get_object store obj_loc (fun obj =>
-      let (store, loc) := Store.add_object store (make_prop_list obj)
-      in result_value store loc
+Definition eval_ownfieldnames runs c st obj_expr : result :=
+  if_eval_return runs c st obj_expr (fun st obj_loc =>
+    assert_get_object st obj_loc (fun obj =>
+      let (st, loc) := add_object st (make_prop_list obj)
+      in result_value st loc
   ))
 .
 
-Definition eval_label runs c store (label : string) body : result :=
-  if_eval_ter runs c store body (fun store res =>
+Definition eval_label runs c st (label : string) body : result :=
+  if_eval_ter runs c st body (fun st res =>
     match res with
-    | res_value ret => result_value store ret
-    | res_exception exc => result_exception store exc
+    | res_value ret => result_value st ret
+    | res_exception exc => result_exception st exc
     | res_break b v =>
       if (decide(b = label)) then
-        result_value store v
+        result_value st v
       else
-        result_break store b v
+        result_break st b v
     end
   )
 .
-Definition eval_break runs c store (label : string) body : result :=
-  if_eval_return runs c store body (fun store ret =>
-    result_break store label ret
+Definition eval_break runs c st (label : string) body : result :=
+  if_eval_return runs c st body (fun st ret =>
+    result_break st label ret
   )
 .
         
-Definition eval_throw runs c store expr : result :=
-  if_eval_return runs c store expr (fun store loc =>
-    result_exception store loc
+Definition eval_throw runs c st expr : result :=
+  if_eval_return runs c st expr (fun st loc =>
+    result_exception st loc
   )
 .
 
-Definition eval_trycatch runs c store body catch : result :=
-  if_eval_ter runs c store body (fun store res =>
+Definition eval_trycatch runs c st body catch : result :=
+  if_eval_ter runs c st body (fun st res =>
     match res with
     | res_exception exc =>
-      if_eval_return runs c store catch (fun store catch =>
-        apply runs c store catch (exc :: nil)
+      if_eval_return runs c st catch (fun st catch =>
+        apply runs c st catch (exc :: nil)
       )
-    | r => result_res store r
+    | r => result_res st r
     end
   )
 .
 
-Definition eval_tryfinally runs c store body fin : result :=
-  if_eval_ter runs c store body (fun store res =>
+Definition eval_tryfinally runs c st body fin : result :=
+  if_eval_ter runs c st body (fun st res =>
     match res with
-    | res_value x => eval_cont_terminate runs c store fin
+    | res_value x => eval_cont_terminate runs c st fin
     | r =>
-      if_eval_return runs c store fin (fun store catch =>
-        result_res store r
+      if_eval_return runs c st fin (fun st catch =>
+        result_res st r
       )
     end
   )
 .
 
-Definition eval_eval runs c store estr bindings :=
-  if_eval_return runs c store estr (fun store v_estr =>
-    if_eval_return runs c store bindings (fun store v_bindings =>
+Definition eval_eval runs c st estr bindings :=
+  if_eval_return runs c st estr (fun st v_estr =>
+    if_eval_return runs c st bindings (fun st v_bindings =>
       assert_get_string v_estr (fun s =>
-        assert_get_object store v_bindings (fun obj => 
-          match desugar_expr s, Store.envstore_of_obj store obj with
-          | Some e, Some (c', store) => runs_type_eval runs c' store e          
+        assert_get_object st v_bindings (fun obj => 
+          match desugar_expr s, envstore_of_obj st obj with
+          | Some e, Some (c', st) => runs_type_eval runs c' st e          
           | None, _ => result_fail "Parse error"
           | _, None => result_fail "Invalid eval environment"
           end 
@@ -438,8 +437,8 @@ Definition eval_eval runs c store estr bindings :=
 (******** Closing the loop *******)
 
 (* Main evaluator *)
-Definition eval runs c store (e : expr) : result :=
-  let return_value := result_value store in
+Definition eval runs c st (e : expr) : result :=
+  let return_value := result_value st in
   match e with
   | expr_undefined => return_value value_undefined
   | expr_null => return_value value_null
@@ -447,50 +446,50 @@ Definition eval runs c store (e : expr) : result :=
   | expr_number n => return_value (value_number n)
   | expr_true => return_value value_true
   | expr_false => return_value value_false
-  | expr_id s => eval_id runs c store s
-  | expr_if e_cond e_true e_false => eval_if runs c store e_cond e_true e_false
-  | expr_seq e1 e2 => eval_seq runs c store e1 e2
-  | expr_object attrs l => eval_object_decl runs c store attrs l
-  | expr_get_field left_ right_ attributes => eval_get_field runs c store left_ right_ attributes
-  | expr_set_field left_ right_ new_val attributes => eval_set_field runs c store left_ right_ new_val attributes
-  | expr_delete_field left_ right_ => eval_deletefield runs c store left_ right_
-  | expr_let id value body => eval_let runs c store id value body
-  | expr_recc id value body => eval_rec runs c store id value body
-  | expr_set_bang id expr => eval_setbang runs c store id expr
-  | expr_lambda args body => eval_lambda runs c store args body
-  | expr_app f args => eval_app runs c store f args
-  | expr_get_attr attr left_ right_ => eval_getattr runs c store left_ right_ attr
-  | expr_set_attr attr left_ right_ newval => eval_setattr runs c store left_ right_ attr newval
-  | expr_get_obj_attr oattr obj => eval_getobjattr runs c store obj oattr
-  | expr_set_obj_attr oattr obj attr => eval_setobjattr runs c store obj oattr attr
-  | expr_own_field_names e => eval_ownfieldnames runs c store e
+  | expr_id s => eval_id runs c st s
+  | expr_if e_cond e_true e_false => eval_if runs c st e_cond e_true e_false
+  | expr_seq e1 e2 => eval_seq runs c st e1 e2
+  | expr_object attrs l => eval_object_decl runs c st attrs l
+  | expr_get_field left_ right_ attributes => eval_get_field runs c st left_ right_ attributes
+  | expr_set_field left_ right_ new_val attributes => eval_set_field runs c st left_ right_ new_val attributes
+  | expr_delete_field left_ right_ => eval_deletefield runs c st left_ right_
+  | expr_let id value body => eval_let runs c st id value body
+  | expr_recc id value body => eval_rec runs c st id value body
+  | expr_set_bang id expr => eval_setbang runs c st id expr
+  | expr_lambda args body => eval_lambda runs c st args body
+  | expr_app f args => eval_app runs c st f args
+  | expr_get_attr attr left_ right_ => eval_getattr runs c st left_ right_ attr
+  | expr_set_attr attr left_ right_ newval => eval_setattr runs c st left_ right_ attr newval
+  | expr_get_obj_attr oattr obj => eval_getobjattr runs c st obj oattr
+  | expr_set_obj_attr oattr obj attr => eval_setobjattr runs c st obj oattr attr
+  | expr_own_field_names e => eval_ownfieldnames runs c st e
   | expr_op1 op e =>
-    if_eval_return runs c store e (fun store v_loc =>
-      if_result_some (Operators.unary op store v_loc) (fun v_res => result_value store v_res)
+    if_eval_return runs c st e (fun st v_loc =>
+      if_result_some (Operators.unary op st v_loc) (fun v_res => result_value st v_res)
     )
   | expr_op2 op e1 e2 =>
-    if_eval_return runs c store e1 (fun store v1_loc =>
-      if_eval_return runs c store e2 (fun store v2_loc =>
-        if_result_some (Operators.binary op store v1_loc v2_loc) (fun v_res => result_value store v_res)
+    if_eval_return runs c st e1 (fun st v1_loc =>
+      if_eval_return runs c st e2 (fun st v2_loc =>
+        if_result_some (Operators.binary op st v1_loc v2_loc) (fun v_res => result_value st v_res)
     ))
-  | expr_label l e => eval_label runs c store l e
-  | expr_break l e => eval_break runs c store l e
-  | expr_try_catch body catch => eval_trycatch runs c store body catch
-  | expr_try_finally body fin => eval_tryfinally runs c store body fin
-  | expr_throw e => eval_throw runs c store e
-  | expr_eval e bindings => eval_eval runs c store e bindings
-  | expr_hint _ e => eval_cont_terminate runs c store e
-  | expr_dump => result_dump c store
+  | expr_label l e => eval_label runs c st l e
+  | expr_break l e => eval_break runs c st l e
+  | expr_try_catch body catch => eval_trycatch runs c st body catch
+  | expr_try_finally body fin => eval_tryfinally runs c st body fin
+  | expr_throw e => eval_throw runs c st e
+  | expr_eval e bindings => eval_eval runs c st e bindings
+  | expr_hint _ e => eval_cont_terminate runs c st e
+  | expr_dump => result_dump c st
   end
 .
 
 Definition runs_0 := {|
-    runs_type_eval := fun c store _ => result_bottom
+    runs_type_eval := fun c st _ => result_bottom
   |}
 .
 
 Definition runs_S runs := 
-  let wrap {A : Type} (f : runs_type -> ctx -> Store.store -> A) c st : A :=
+  let wrap {A : Type} (f : runs_type -> ctx -> store -> A) c st : A :=
     f runs c st
   in {|
     runs_type_eval := wrap eval
